More. Finish [pstore_collect].

theories/common/treemap.v
@@ -18,26 +18,28 @@ Section treemap_rooted.
   Implicit Types ϵ : N * E.
   Implicit Types tree : treemap N E.
 
-  Inductive treemap_path tree dst : N → list E → Prop :=
+  Inductive treemap_path tree root : N → list E → Prop :=
     | treemap_path_nil :
-        treemap_path tree dst dst []
+        treemap_path tree root root []
     | treemap_path_cons {node1} ϵ node2 edge edges :
         tree !! node1 = Some ϵ →
         ϵ.1 = node2 →
         ϵ.2 = edge →
-        treemap_path tree dst node2 edges →
-        treemap_path tree dst node1 (edge :: edges).
+        treemap_path tree root node2 edges →
+        treemap_path tree root node1 (edge :: edges).
   #[local] Hint Constructors treemap_path : core.
 
   Definition treemap_rooted tree root :=
-    ∀ node,
-    is_Some (tree !! node) →
-      ∃ edges,
-      treemap_path tree root node edges.
+    tree !! root = None ∧
+      ∀ node,
+      is_Some (tree !! node) →
+        ∃ edges,
+        treemap_path tree root node edges.
 
   Lemma treemap_rooted_empty root :
     treemap_rooted ∅ root.
   Proof.
+    split; first done.
     intros node []%(lookup_empty_is_Some (A := N * E)).
   Qed.
 
@@ -52,6 +54,29 @@ Section treemap_rooted.
       ∃ edges,
       treemap_path tree root node edges.
   Proof.
-    auto.
+    rewrite /treemap_rooted. naive_solver.
+  Qed.
+
+  Lemma treemap_path_is_nil tree root edges :
+    treemap_rooted tree root →
+    treemap_path tree root root edges →
+    edges = [].
+  Proof.
+    intros (Hlookup_root & _) Hpath.
+    invert Hpath. done.
+  Qed.
+  Lemma treemap_path_is_cons tree root node edges :
+    treemap_rooted tree root →
+    treemap_path tree root node edges →
+    node ≠ root →
+      ∃ node' edge edges',
+      edges = edge :: edges' ∧
+      tree !! node = Some (node', edge) ∧
+      treemap_path tree root node' edges'.
+  Proof.
+    intros Hrooted Hpath Hnode.
+    invert Hpath as [| ? []]. naive_solver.
   Qed.
 End treemap_rooted.
+
+#[global] Opaque treemap_rooted.
